In this [[b. Injectivity of Maximum-area Sofas/10. Convex Bodies/10. Surface Area Measure]], we will prove an that relates the vertices $v_K^{\pm}(t)$ of a convex body $K$ to its surface area measure $\sigma_K$.

That is, if we write the coordinates of $v_K^+(t)$ as $(x(t), y(t))$, then the Lebesgue-Stieltjes measure $dx$ and $dy$ of $x(t)$ and $y(t)$ are $-\sin t \cdot \sigma_K(dt)$ and $\cos t \cdot \sigma_K(dt)$ respectively. Note that $dx$ and $dy$ are well-defined because $v_K^+(t)$ is of bounded variation ([[xx. Mamikon's Theorem/05. Vertex and support function#^thm-vertex-bounded-variation]]) and right-continuous ([[xx. Mamikon's Theorem/05. Vertex and support function#^cor-vertex-right-continuous]]).

> __Theorem [boundary-measure].__ Consider $u_t$ as the function $u(t) := u_t$ so that $u : I \to \mathbb{R}^2$. For every interval $I = (a, b]$ in $S^1$ of length $\leq 2\pi$, we have ^thm-boundary-measure
$$
\mathrm{d} v_K^{+} = u \, \sigma
$$
> where both sides are pairs of Borel measures on $I$. Consequently, we have
$$
\int_{t \in I} p(t) \, \mathrm{d} v_K^+(dt) = \int_{t \in I} u_t\,\sigma(dt)
$$
> for any Borel function $p$ on $X$.

> __Definition [measure-restriction].__  ^def-measure-restriction

_Proof._ For any measure $\sigma$ on $S^1$ and a Borel subset $A$ of $S^1$, define the _restriction_ $\sigma|_A$ of $\sigma$ to $A$ as the measure on $S^1$ defined as $\sigma|_A(X) = \sigma(A \cap X)$.

First we observe that the equality holds when $K$ is a polygon. In this case, for every $t$ the value $\sigma_K(t)$ is nonzero if and only if it measures the length of a proper edge $e_K(t)$. So the right-hand side measures the sum of all vectors from vertex $v_K^-(t)$ to $v_K^+(t)$ along the proper edges $e_K(t)$ with angles $t \in (t_1, t_2]$. The sum in the right-hand side is then the vector from $v_K^+(t_1)$ to $v_K^+(t_2)$, justifying the equality for polygon $K$.

$S_1(K, -)$ or $S_K$ in p464 of [[@schneider_2013]].

Now we prove the equality for general $K$. As in the proof of Theorem 8.3.3, p466 of [[@schneider_2013]], we can take a series $K_1, K_2, \dots$ of polygons converging to $K$ in the Hausdorff distance such that $e_{K_n}(t_i) = e_{K}(t_i)$ for all $n = 1, 2, \dots$ and $i = 1, 2$. In particular, we have $v_{K_n}^{\pm}(t_i) = v_{K}^{\pm}(t_i)$ and $\sigma_{K_n}(\{t_i\}) = \sigma_{K}(\{t_i\})$ for all $n = 1, 2, \dots$ and $i = 1, 2$. By Theorem 4.2.1, p212 of [[@schneider_2013]], the measures $\sigma_{K_n}$ converge to $\sigma_K$ weakly as $n \to \infty$.

Define $U$ as the open set $S^1 \setminus \left\{ t_1, t_2 \right\}$ of $S$, and $V$ as the open interval $(t_1, t_2)$ of $S^1$. Define $u_n$ and $u$ as the restriction of $\sigma_{K_n}$ and $\sigma_K$ to $U$, then $u_n$ converges to $u$ weakly as $n \to \infty$ because $\sigma_{K_n}(\{t_i\}) = \sigma_{K}(\{t_i\})$ for $i = 1, 2$. Define $\lambda_n$ and $\lambda$ as the restriction of $\sigma_{K_n}$ and $\sigma_K$ to $V$. We want to prove that $\lambda_n \to \lambda$ weakly as $n \to \infty$. Take any continuity set $X$ of $\lambda$ so that $\lambda(\partial X) = 0$ and thus $u(\partial X \cap V) = 0$. Because $\partial(X \cap V) \subseteq (\partial X \cap V) \cup \partial V$, and both $u(\partial X \cap V)$ and $u(\partial V)$ are zero, the set $X \cap V$ is a continuity set of $u$. So $u_n(X \cap V) \to u(X \cap V)$ and thus $\lambda_n(X) \to \lambda(X)$ as $n \to \infty$. This completes the proof that $\lambda_n \to \lambda$ weakly as $n \to \infty$.

We finally take the limit $n \to \infty$ to the equality
$$
v_{K_n}^+(t_2) - v_{K_n}^+(t_1) = \int_{t \in (t_1, t_2]} v_t \, \sigma_{K_n}(dt)
$$
for polygons $K_n$. The left-hand side is equal to $v_K^+(t_2) - v_K^+(t_1)$ by the way how we took $K_n$. The right-hand side is equal to
$$
(v_{K_n}^+(t_2) - v_{K_n}^-(t_2)) + \int_{t \in S^1} v_t \, \lambda_n(dt)
$$
and by $v_{K_n}^{\pm}(t_i) = v_{K}^{\pm}(t_i)$ and the weak convergence $\lambda_n \to \lambda$, the expression converges to
$$
(v_{K}^+(t_2) - v_{K}^-(t_2)) + \int_{t \in S^1} v_t \, \lambda(dt) = \int_{t \in (t_1, t_2]} v_t\, \sigma_{K}(dt)
$$
thus completing the proof for general $K$. â–¡