In this section, we calculate the directional derivative $D_K\mathcal{A}_1$ of $\mathcal{A}_1$ at any $K \in \mathcal{K}_{\pi/2}$. As $\mathcal{A}_1(K) = \left| K \right| - \mathcal{I}(\mathbf{x}_K)$, we calculate the directional derivative of $|K|$ and $\mathcal{I}(\mathbf{x}_K)$ separately.

> __Theorem [convex-body-area-variation].__ Let $K$ and $K'$ be arbitrary convex bodies. Then we have the following. ^thm-convex-body-area-variation
$$
D_K\left| - \right|(K') = \left< p_{K'} - p_K , \beta_K \right>_{S^1} 
$$

_Proof._ For any convex body $K$ we have $|K| = V(K, K)$ where $V$ is the mixed volume of two planar convex bodies. Also note that $V(K_1, K_2) = V(K_2, K_1)$. So by [[15. Directional Derivative#^lem-quadratic-variation]] □

> __Theorem [curve-area-variation].__ Let $\mathbf{x}_1, \mathbf{x}_2 : [t_a, t_b] \to \mathbb{R}$ be arbitrary rectifiable curves with the same domain $[t_a, t_b]$. Then we have the following. ^thm-curve-area-variation
$$
D_{}
$$

_Proof._ 
□

We also calculate the differentiation of $\mathbf{x}_K(t)$ for any cap $K \in \mathcal{K}_\omega$.

> __Theorem [inner-corner-deriv].__ For any cap $K \in \mathcal{K}_\omega$, the right derivative of the outer and inner corner $\mathbf{y}_K(t)$ exists for any $0 \leq t < \omega$ and is equal to the following. ^thm-inner-corner-deriv
$$
\begin{align*}
	\partial^+ \mathbf{y}_K(t) = -g_K^+(t) u_t + h_K^+(t) v_t \qquad \partial^+ \mathbf{x}_K(t) = -(g_K^+(t) - 1) u_t + (h_K^+(t) - 1) v_t
\end{align*}
$$
> Likewise, $\mathbf{v}_K^- (t)$ exists for all $0 < t \leq \omega$ and is equal to the following.
$$
\begin{align*}
	\partial^- \mathbf{y}_K(t) = -g_K^-(t) u_t + h_K^-(t) v_t \qquad \partial^+ \mathbf{x}_K(t) = -(g_K^-(t) - 1) u_t + (h_K^-(t) - 1) v_t
\end{align*}
$$

_Proof._ Fix an arbitrary cap $K$ and omit the subscript $K$. Take any $0 \leq t < \omega$ and set $s = t + \delta$ for sufficiently small and arbitrary $\delta > 0$. We simplify $\partial^+ \mathbf{y}(t) = \lim_{\delta \rightarrow 0^+}(\mathbf{y}(s) - \mathbf{y}(t)) / \delta$. Define $A_{t, s} = a(t) \cap a(s)$. Since $A_{t, s}$ is on the lines $a(t)$ and $a(s)$, it satisfies both $A_{t, s} \cdot u_t = \mathbf{y}(t) \cdot u_t$ and $A_{t, s} \cdot u_s = \mathbf{y}(s) \cdot u_s$. Rewrite $u_s = \cos \delta \cdot u_t + \sin \delta \cdot v_t$ on the second equation and we have
$$
\begin{align*}
	A_{t, s} \cos \delta \cdot u_t + A_{t, s} \sin \delta \cdot v_t =  	\cos \delta (\mathbf{y}(s) \cdot u_t) + \sin \delta (\mathbf{y}(s) \cdot v_t).
\end{align*}
$$
Group by $\cos \delta$ and $\sin \delta$ and substitute $A_{t, s} \cdot u_t$ with first equation then
$$ \cos \delta (\mathbf{y}(s) \cdot u_t - \mathbf{y}(t) \cdot u_t)
	= \sin \delta (A_{t, s}  (s) \cdot v_t - \mathbf{y}(s) \cdot v_t) .
	$$
Divide by $\delta$ and send $\delta \to 0^+$. Observe that $A_{t, s} \to A^+(t)$. We get
$$ (\partial^+ \mathbf{y}(t)) \cdot u_t  = (A^+(t) - \mathbf{y}(t)) \cdot v_t = - g^+(t)$$
as $g^+(t) = (\mathbf{y}(t) - A^+(t)) \cdot v_t$. A similar argument can be applied to show $(\partial^+ \mathbf{y}(t)) \cdot v_t = h^+(t)$ and thus the first equation of the theorem. The right derivative of $\mathbf{x}_K(t)$ comes from $\mathbf{x}_K(t) = \mathbf{y}_K(t) - u_t - v_t$. A symmetric argument calculates the left derivative of the outer and inner corner. □

> __Definition [i-cap].__ For any cap $K$, define $i_K : J_\omega \to \mathbb{R}$ as $i_K(t) = h_K^+(t) - 1$ and $i_K(t + \pi / 2) = g^+_K(t) - 1$ for $t \in [0, \omega]$. Define $\iota_K$ as the measure on $J_\omega$ derived from the density function $i_K$. That is, $\iota_K(dt) = i_K(t) dt$. ^def-i-cap
 
> __Theorem [variation-a1].__ Let $K_1$ and $K_2$ be two caps in $\mathcal{K}_\omega$. Define $K= (1-\lambda)K_1 + \lambda K_2$ as the interpolation between $K_1$ and $K_2$ with $0 \leq \lambda \leq 1$. Then we have the following calculation. ^thm-variation-a1
$$
\left. \frac{d}{d\lambda} \right|_{\lambda = 0} \mathcal{A}_1(K)
= \left< p_{K_2} - p_{K_1}, \beta_{K_1} - \iota_{K_1} \right>_{J_\omega}
$$

_Proof._ We start from $\mathcal{A}_1(K) = |K| - \mathcal{I}(\mathbf{x}_K)$. By applying [[15. Directional Derivative#^thm-convex-body-area-variation]] to the first term and applying [[15. Directional Derivative#^thm-curve-area-variation]] to the second term, we get the following.
$$
\left. \frac{d}{d\lambda} \right|_{\lambda = 0} \mathcal{A}_1(K)
= \int_{t \in [0, \omega]} (p_{K_2} (t) - p_{K_1}(t)) \beta_{K_1} (dt) - 
\int_0^\omega (\mathbf{x}_{K_2} - \mathbf{x}_{K_1}) \times d\mathbf{x}_{K_1}(t)
$$
Let's focus on the second term more. We write each vector as linear combinations of $u_t$ and $v_t$. This follows from definition of $\mathbf{x}_K$.
$$
\mathbf{x}_{K_2} - \mathbf{x}_{K_1} = (p_{K_2} (t) - p_{K_1} (t)) u_t + 
(p_{K_2} (t + \pi / 2) - p_{K_1} (t + \pi / 2))) v_t
$$
And [[01. Space of Caps#^thm-inner-corner-deriv]] gives the following almost everywhere.
$$
\mathbf{x}'_{K_1} = \mathbf{v}_{K_1}(t) = -(g_{K_1}^+(t) - 1) \cdot u_t + (h_{K_1}^+(t) - 1) \cdot v_t
$$
So the cross-product $(\mathbf{x}_{K_2} - \mathbf{x}_{K_1}) \times \mathbf{x}'_{K_1}$ is equal to the following almost everywhere.
$$
(h_K^+(t) - 1) (p_{K_2} (t) - p_{K_1} (t)) + (g_K^+(t) - 1) (p_{K_2} (t + \pi / 2) - p_{K_1} (t + \pi / 2)))
$$
Using [[#^def-i-cap]], the second integral can be expressed more concisely.
$$
\int_0^\omega (\mathbf{x}_{K_2} - \mathbf{x}_{K_1}) \times d\mathbf{x}_{K_1}(t) = 
\int_{t \in J_\omega} (p_{K_2} (t) - p_{K_1}(t)) i_{K_1}(t) dt
$$
We get the original equation by plugging this back to the equation for $\left. \frac{d}{d\lambda} \right|_{\lambda = 0} \mathcal{A}_1(K)$. □


> __Proposition [cap-corner-curve-functional].__ Let $\phi_1, \phi_2$ be two angles. Define $I$ as a subinterval of $J$. Then $\mathcal{I}(\mathbf{x}_K|_I) = \left< p_K, \iota_K \right>_{I}$ ^pro-cap-corner-curve-functional