We now solve for the maximizer $K = K_{\max, 1}$ of our concave quadratic upper bound $\mathcal{A}_1(K)$. We do this _a priori_ by solving for the cap $K$ where $\beta_{K} = \iota_{K}$ on the set $[0, \pi] \setminus \left\{ \pi/2 \right\}$. Once the equation $\beta_K = \iota_K$ is solved, then for every other cap $K'$ we have $D\mathcal{A}_1(K; K') = 0$ by [[15. Directional Derivative of A1#^thm-variation-a1]] as we have $\beta_{K} = \iota_{K}$ on $[0, \pi] \setminus \left\{ \pi/2 \right\}$ and $p_{K'}(\pi/2) = p_K(\pi/2) = 1$. Then by [[02. Space of Caps#^thm-quadratic-variation]] the cap $K$ attains the maximum value of $\mathcal{A}_1$.

We need some preparation to solve for the equation $\beta_K = \iota_K$ on $[0, \pi] \setminus \left\{ \pi/2 \right\}$. From now on, let $K \in \mathcal{K}_{\pi/2}$ be an arbitrary cap. We will use the arm lengths $g_K^{\pm}(t)$ and $h_K^{\pm}(t)$ as our main tool for caculation.

From [[03. Surface Area Measure#^thm-surface-area-measure-vertex]] with $a = t$ and $b = t + \pi/2$, we have the following.

> __Lemma [arm-length-integral].__ For every $t \in [0, \pi/2]$ we have the followings. ^lem-arm-length-integral
$$
g_K^+(t) = \int_{(t, t + \pi/2]} \cos(u - t) \, \beta_K(du) \qquad g_K^-(t) = \int_{[t, t + \pi/2]} \cos(u - t) \, \beta_K(du)
$$
$$
h_K^+(t) = \int_{[t, t + \pi/2]} \sin(u - t) \, \beta_K(du) \qquad h_K^-(t) = \int_{[t, t + \pi/2)} \sin(u - t) \, \beta_K(du)
$$

For most $t \in (0, \pi/2)$, the values $g_K^+(t)$ and $g_K^-(t)$ (resp. $h_K^+(t)$ and $h_K^-(t)$) are equal and we will denote the common value by dropping their signs.

> __Definition [arm-length-unsinged].__ For any angle $t \in (0, \pi/2)$, if $g_K^+(t) = g_K^-(t)$ (resp. $h_K^+(t) = h_K^-(t)$) then we simply denote the matching value as $g_K(t)$ (resp. $h_K(t)$). Note that the condition holds if and only if $\beta_K(\left\{ t \right\}) = 0$ (resp. $\beta_K(\left\{ t + \pi/2 \right\})$) by [[20. Maximizer of A1#^lem-arm-length-integral]]. ^def-arm-length-unsinged

Now we calculate the derivatives of $g_K(t)$ and $h_K(t)$.

> __Theorem [arm-length-derivative].__ Assume that there is a open interval $U$ in $(0, \pi/2)$ and a continuous function $f : U \cup \left( U + \pi/2 \right) \to \mathbb{R}$ such that the measure $\beta_K$ has density function $f$ on $U \cup (U + \pi/2)$. That is, we have $\beta_K(X) = \int_X f(x)\,dx$ for every measurable $X \subseteq U \cup (U + \pi/2)$. Then we have $g_{K}'(t) = -f(t) + h_{K}(t)$ and $h_K'(t) = f(t_0 + \pi/2) - g_K(t)$ for every $t \in U$. ^thm-arm-length-derivative

_Proof._ We have the followings for every $t \in U$ by [[20. Maximizer of A1#^lem-arm-length-integral]].
$$
g_{K}(t) = \int_{t}^{t+\pi/2} \cos \left( u - t \right) \beta_K(du)
$$
$$
h_{K}(t) = \int_{t}^{t+\pi/2} \sin \left( u - t \right) \beta_K(du)
$$
Differentiate those at $t \in U$ using Leibniz integral rule to get the following.
$$
g_{K}'(t) = -f(t) + \int_{t}^{t+\pi/2} \sin (u-t)\, \beta_K(du) = -f(t) + h_{K}(t) 
$$
$$
h_{K}'(t) = f\left( t + \pi/2 \right) - \int_{t}^{t+\pi/2} \cos (u-t)\, \beta_K(du) = f(t + \pi/2) - g_{K_1}(t)
$$
□

The following theorem solves the equation $\beta_K = \iota_K$ on any open interval $(t_1, t_2) \cup (t_1 + \pi/2, t_2 + \pi/2)$. Note that this equation is a mesure-theoretic version of (ODE3) in Theorem 2 of [[@romikDifferentialEquationsExact2018]] generalized to arbitrary caps.

> __Theorem [balanced-ACx].__ Let $K \in \mathcal{K}_{\pi/2}$ be any cap. Let $0 \leq t_1 < t_2 < \pi/2$ be two arbitrary angles. Then the followings are equivalent. ^thm-balanced-ACx
> 
> - We have $\beta_{K} = \iota_{K}$ on the set $(t_1, t_2) \cup (t_1 + \pi/2, t_2 + \pi/2)$
> - We have $\beta_K(dt) = (a_0 - t) dt$ and $\beta_K(dt + \pi/2) = (c_0 + t) dt$ on the interval $t \in (t_1, t_2)$ where $a_0 = h_K^+(t_1) + t_1 - 1$ and $c_0 = g_K^+(t_1) - t_1 - 1$.
> 
> Moreover, for such $K$ we have $g_K(t) = g_K^+(t_1) + (t - t_1)$ and $h_K(t) = h_K^+(t_1) - (t - t_1)$ for $t \in (t_1, t_2)$, and $g_K^-(t_2) - g_K^+(t_1) = t_2 - t_1$ and $h_K^-(t_2) - h_K^+(t_1) = -(t_2 - t_1)$ consequently.

_Proof._ Assume that $\beta_K = \iota_K$ on the set $X = (t_1, t_2) \cup (t_1 + \pi/2, t_2 + \pi/2)$. Since the measure of $\beta_K$ is zero for every point of $X$, by [[20. Maximizer of A1#^def-arm-length-unsinged]] we have $g_K(t) = g^\pm_K(t)$ and $h_K(t) = h_K^{\pm}(t)$ for every $t \in (t_1, t_2)$. Also, by applying dominating convergence theorem to [[20. Maximizer of A1#^lem-arm-length-integral]], the functions $g_K(t)$ and $h_K(t)$ are continuous with respect to every $t \in (t_1, t_2)$. Now we can apply [[20. Maximizer of A1#^thm-arm-length-derivative]] to $K$ as $\beta_K = \iota_K$ has the continuous density function $i_K$ on $X$. For every $t \in (0, \pi/2)$, we have the followings by [[20. Maximizer of A1#^thm-arm-length-derivative]] and [[15. Directional Derivative of A1#^def-i-cap]].
$$
\begin{gather}
g_{K}'(t) = -i_K(t) + h_{K}(t) = 1 \\
h_K'(t) = i_K(t + \pi/2) - g_K(t) = -1
\end{gather}
$$
As $g_K(t) \to g_K^+(t_1)$ as $t \to t_1^+$, we have $g_K(t) = g_K^+(t_1) + (t - t_1)$ for every $t \in (t_1, t_2)$. Likewise, as $h_K(t) \to h_K^+(t_1)$ as $t \to t_1^+$, we have $h_K(t) = h_K^+(t_1) - (t - t_1)$ for every $t \in (t_1, t_2)$. By [[15. Directional Derivative of A1#^def-i-cap]], we have $i_K(t) = h_K(t) - 1 = h_K^+(t_1) - (t - t_1) - 1$ and $i_K(t + \pi/2) = g_K(t) - 1 = g_K^+(t_1) + (t - t_1) - 1$. As $\beta_K(dt) = i_K(t)dt$ on $X$, we have $\beta_K(dt) = (a_0 - t) dt$ and $\beta_K(dt + \pi/2) = (c_0 + t) dt$ where $a_0 = h_K^+(t_1) + t_1 - 1$ and $c_0 = g_K^+(t_1) - t_1 - 1$.

Now let $K$ be any cap satisfying $\beta_K(dt) = (a_0 - t) dt$ and $\beta_K(dt + \pi/2) = (c_0 + t) dt$ on the interval $t \in (t_1, t_2)$ where $a_0 = h_K^+(t_1) + t_1 - 1$ and $c_0 = g_K^+(t_1) - t_1 - 1$. Then by [[20. Maximizer of A1#^thm-arm-length-derivative]] we have the followings.
$$
\begin{gather}
g_{K}'(t) = -(a_0 - t) + h_{K}(t) \\
h_K'(t) = (c_0 + t) - g_K(t)
\end{gather}
$$
We have $g_K(t) \to g_K^+(t_1)$ and $g_K'(t) = -(a_0 - t) + h_K(t) \to -(h_K^+(t_1) - 1) + h_K(t_1) = 1$ as $t \to t_1^+$. Likewise, $h_K(t) \to h_K^+(t_1)$ and $h_K'(t) \to -1$ as $t \to t_1^+$. So the unique solutions $g_K(t)$ and $h_K(t)$ satisfying the ODEs above are $g_K(t) = g_K^+(t_1) + (t - t_1)$ and $h_K(t) = h_K^+(t_1) - (t - t_1)$ for $t \in (t_1, t_2)$, completing the proof. □

With [[20. Maximizer of A1#^thm-balanced-ACx]], we can now solve for the equation $\beta_K = \iota_K$ on $[0, \pi] \setminus \left\{ \pi/2 \right\}$ with $t_1 = 0$ and $t_2 = \pi/2$. Let $K$ be a solution, then it should be that $g_K(0) = 1$ and $h_K(\pi/2) = 1$ as $\beta_K(\left\{ 0 \right\}) = \beta_K(\left\{ \pi \right\}) = 0$. So by [[20. Maximizer of A1#^thm-balanced-ACx]] we should have $\beta_K(dt) = (\pi/2 - t) dt$ and $\beta_K(dt + \pi/2) = t dt$ on the set $t \in (0, \pi/2)$. We also have $g_K^-(\pi/2) = 1 + \pi/2$. Another calculation by [[20. Maximizer of A1#^lem-arm-length-integral]] shows $g_K^+(\pi/2) = \int_0^{\pi/2} t \cos t\, dt = \pi / 2 - 1$. So we also have $\beta_K(\left\{ \pi/2 \right\}) = 2$ as well (note that on the other hand we have $\iota_K(\left\{ \pi/2 \right\}) = 0$). So the solution $K$ should be the following cap.

> __Definition [maximum-presofa-a1].__ Define the cap $K = K_{\max, 1} \in \mathcal{K}_{\pi/2}$ as the cap with following boundary measure $\beta_{K}$ and $p_K(0) = 1$. ^def-maximum-presofa-a1
> 
> - $\beta_K(\left\{ \pi/2 \right\}) = 2$
> - $\beta_{{K}}(dt) = (\pi/2 -t)dt$ on $t \in [0, \pi/2)$ and $\beta_{K}(dt) = (t - \pi/2)dt$ on $t \in (\pi/2, \pi]$.

To justify the existence of such $K = K_{\max, 1}$ we can use [[03. Surface Area Measure#^thm-cap-from-boundary-measure]]. By [[03. Surface Area Measure#^thm-cap-from-boundary-measure]], we only need to check $\int_0^{\pi/2} \cos(t) (\pi/2 - t) \, dt = 1$ which is true by calculation. So there is $K_{\max, 1}$ satisfying [[20. Maximizer of A1#^def-maximum-presofa-a1]].

By [[20. Maximizer of A1#^thm-balanced-ACx]] we have $\beta_K = \iota_K$ on $[0, \pi] \setminus \left\{ \pi/2 \right\}$ for $K = K_{\max, 1}$ indeed, and so by [[02. Space of Caps#^thm-quadratic-variation]] we get the following.

> __Theorem [maximum-presofa-a1].__ The cap $K_{\max, 1}$ maximizes $\mathcal{A}_1 : \mathcal{K}_{\pi/2} \to \mathbb{R}$. ^thm-maximum-presofa-a1

The maximum value of $\mathcal{A}_1$ is very close to the area $\mu_G = 2.2195\dots$ of Gerver's sofa.

> __Theorem [maximum-presofa-a1-area].__ The maximum value $\mathcal{A}_1(K_{\max, 1})$ of $\mathcal{A}_1$ is $1 + \pi^2/8 = 2.2337\dots$.  ^thm-maximum-presofa-a1-area

_Proof._ (TODO: plug in $\omega = \pi/2$ for this general calculation with arbitrary rotation angle) If $\omega = \pi/2$, let $p_\omega = (0, 1)$. Let $\tau = (\pi/2-\omega)/2$. Then we have $p_\omega = (\tan(\tau), 1)$ for any angle $\omega \leq \pi/2$. Note that $K_1$ has mirror symmetry along the line segment connecting $(0, 0)$ and $p_\omega$.

Let us compute the value of $p_{K_1}(t)$ for $t \in [0, \omega]$. 
$$
\begin{align*}
p_{K_1}(t) - p_\omega \cdot u_t & = (A^-_{K_1}(t) - p_\omega) \cdot u_t =  \\
& = \sin(\omega - t) + \int_{t_0 \in [t, \omega] } (\omega - t_0) \sin \left( t_0 - t \right) \, dt_{0} \\
& = \omega - t
\end{align*}
$$
So $p_{K_1}(t) = \omega - t + p_{\omega} \cdot u_t$ on $t \in [0, \omega]$. By symmetry, $p_{K_1}(t) = t - \pi/2 + p_\omega \cdot u_t$ on $t \in [\pi/2, \omega + \pi/2]$. Now use the mirror symmetry to calculate half the area of $K_1$.
$$
\begin{align*}
\frac{1}{2} \int_{t \in [0, \omega]} p_{K_1}(t) \, \beta(dt) & = 
\frac{1}{2} + \frac{1}{2} \int_{t \in [0, \omega]} \left( \omega - t + p_\omega \cdot u_t \right)  (\omega-t) \, dt \\
& = \frac{1}{2} + \frac{1}{2} \left( \omega^3 / 3 + p_\omega \cdot (1 - \cos(\omega), \omega - \sin(\omega)) \right) 
\end{align*}
$$
So we have the following.
$$
\begin{align*}
|K_1| & = 1 + \omega^3 / 3 + p_\omega \cdot (1 - \cos \omega, \omega - \sin \omega) \\
& = \omega^3/3 + \omega + \cot\left( \pi/4 + \omega/2 \right)
\end{align*}
$$

Next, we compute the area of the niche $I(\mathbf{x}_{K_1})$. We have 
$$
\mathbf{x}_{K_1}(t) = (p_{K_1}(t) - 1)u_t + (p_{K_1}(t + \pi/2) - 1) v_t
$$
and
$$
\mathbf{x}'_{K_1} = -(g_{K_1}^+(t) - 1) \cdot u_t + (h_{K_1}^+(t) - 1) \cdot v_t = 
- t \cdot u_t + (\omega - t) \cdot v_t
$$
so
$$
\begin{align*}
I(\mathbf{x}_{K_1}) & = \frac{1}{2} \int_0^\omega (p_{K_1}(t) - 1)(\omega - t) + (p_{K_1}(t+\pi/2) - 1) t \, dt  \\
& = \frac{1}{2} \int_0^\omega (\omega - t + p_{\omega} \cdot u_t - 1) (\omega - t) \, dt + 
\frac{1}{2} \int_0^\omega (t + p_{\omega} \cdot v_t - 1) t \, dt \\
& = \omega^3 / 3 - \omega^2 / 2 + (-1 + \omega + \cot\left( \pi/4 + \omega/2 \right) )
\end{align*}
$$
Finally, we compute $\mathcal{A}_1(K_1) = |K_1| - I(\mathbf{x}_{K_1}) = 1 + \omega^2 / 2$. □